verification/tests/LaunchpadDistributeTokensTests.dfy
@@ -1,0 +1,42 @@
+module LaunchpadDistributeTokensTests {
+  import opened Config
+  import opened Investments
+  import opened Distribution
+  import opened Launchpad
+  import opened LaunchpadUtils
+
+  function DistributeTokensTest(): bool {
+    var stakeHolder1 := StakeholderProportion(IntentAccount("stakeHolder1.testnet"), 50000);
+    var stakeHolder2 := StakeholderProportion(IntentAccount("stakeHolder2.testnet"), 25000);
+    var stakeHolder3 := StakeholderProportion(IntentAccount("stakeHolder3.testnet"), 1000);
+    var stakeHolder4 := StakeholderProportion(IntentAccount("stakeHolder4.testnet"), 1000);
+    var distr := DistributionProportions(IntentAccount("solver.testnet"), 100000, [stakeHolder1, stakeHolder2, stakeHolder3, stakeHolder4]);
+    assert distr.isUnique();
+
+    var cfg := InitConfig()
+               .(totalSaleAmount := 377000)
+               .(distributionProportions := distr);
+    var lp := InitLaunchpad(cfg);
+    assert lp.IsInitState();
+
+    var (lp1, amount1, weight1, refund1) := lp.DepositSpec(cfg.saleTokenAccountId, cfg.totalSaleAmount, IntentAccount(cfg.saleTokenAccountId), 100);
+    assert amount1 == cfg.totalSaleAmount;
+    assert lp1.IsOngoing(NOW);
+
+    var alice := "alice.testnet";
+    var (lp2, _, _, _) := lp1.DepositSpec(alice, 200000, IntentAccount(alice), NOW);
+    assert lp2.totalDeposited == 200000;
+    assert lp2.totalSoldTokens == 200000;
+    assert lp2.investments[IntentAccount(alice)] == InvestmentAmount(200000, 200000, 0);
+    assert lp2.IsSuccess(cfg.endDate);
+
+    var lp3 := lp2.DistributeTokensSpec(Intents, cfg.endDate);
+
+    assert |lp3.distributedAccounts| == 3;
+    assert cfg.distributionProportions.solverAccountId in lp3.distributedAccounts;
+    // assert stakeHolder1.account in lp3.distributedAccounts;
+    // assert stakeHolder2.account in lp3.distributedAccounts;
+
+    true
+  }
+}
